seplogic: add split lang and rgsep + local and shared liftings

RGLogic.thy
@@ -1,5 +1,5 @@
 theory RGLogic
-  imports SepAlgInstances
+  imports Lang
 begin
 
 section \<open> rely/guarantee helpers \<close>
@@ -87,6 +87,36 @@ lemma wssa_of_pred_Times_eq[simp]:
 lemma sp_rely_of_pred_Times_eq[simp]:
   \<open>sswa r (p \<times>\<^sub>P q) = (p \<times>\<^sub>P sp r\<^sup>*\<^sup>* q)\<close>
   by (force simp add: rel_Times_def pred_Times_def sp_def split: prod.splits)
+
+subsection \<open> Local and shared predicate lifting \<close>
+
+abbreviation(input) local_pred
+  :: \<open>('a::perm_alg \<Rightarrow> bool) \<Rightarrow> ('a \<times> 'b \<Rightarrow> bool)\<close> (\<open>\<L>\<close>)
+  where
+    \<open>\<L>(p) \<equiv> p \<circ> fst\<close>
+
+abbreviation(input) shared_pred
+  :: \<open>('b::perm_alg \<Rightarrow> bool) \<Rightarrow> ('a \<times> 'b \<Rightarrow> bool)\<close> (\<open>\<S>\<close>)
+  where
+    \<open>\<S>(p) \<equiv> p \<circ> snd\<close>
+
+lemma wssa_ignore_local[simp]:
+  \<open>wssa r (\<L> pl) = \<L> pl\<close>
+  by (fastforce simp add: wlp_def fun_eq_iff sepconj_conj_def)
+
+lemma sswa_ignore_local[simp]:
+  \<open>sswa r (\<L> pl) = \<L> pl\<close>
+  \<open>sswa r (\<L> pl \<^emph>\<and> q) = \<L> pl \<^emph>\<and> sswa r q\<close>
+  \<open>sswa r (p \<^emph>\<and> \<L> ql) = sswa r p \<^emph>\<and> \<L> ql\<close>
+  by (force simp add: sp_def fun_eq_iff sepconj_conj_def)+
+
+lemma wssa_over_shared:
+  \<open>wssa r (\<S> ps) = \<S> (wlp r\<^sup>*\<^sup>* ps)\<close>
+  by (force simp add: wlp_def fun_eq_iff sepconj_conj_def)
+
+lemma sswa_over_shared:
+  \<open>sswa r (\<S> ps) = \<S> (sp r\<^sup>*\<^sup>* ps)\<close>
+  by (force simp add: sp_def fun_eq_iff sepconj_conj_def)
 
 
 section \<open> Framed step relation \<close>
@@ -192,340 +222,6 @@ lemma (in sep_alg) sep_alg_framed_subresource_rel_iff:
   done
 
 
-section \<open> Language Definition \<close>
-
-subsection \<open> Commands \<close>
-
-datatype 'a comm =
-  Skip
-  | Seq \<open>'a comm\<close> \<open>'a comm\<close> (infixr \<open>;;\<close> 75)
-  | Par \<open>'a comm\<close> \<open>'a comm\<close> (infixr \<open>\<parallel>\<close> 65)
-  | Indet \<open>'a comm\<close> \<open>'a comm\<close> (infixr \<open>\<^bold>+\<close> 65)
-  | Endet \<open>'a comm\<close> \<open>'a comm\<close> (infixr \<open>\<box>\<close> 65)
-  | Atomic \<open>'a \<Rightarrow> 'a \<Rightarrow> bool\<close>
-  | Iter \<open>'a comm\<close> (\<open>DO (_) OD\<close> [0] 999)
-\<comment> \<open> loops are represented by (least) fixed points. Fixed point variables are done in de Brijn
-style. \<close>
-  | Fix \<open>'a comm\<close> (\<open>\<mu>\<close>)
-  | FixVar nat
-
-subsection \<open> substitution \<close>
-
-primrec map_fixvar :: \<open>(nat \<Rightarrow> nat) \<Rightarrow> 'a comm \<Rightarrow> 'a comm\<close> where
-  \<open>map_fixvar f Skip = Skip\<close>
-| \<open>map_fixvar f (c1 ;; c2) = map_fixvar f c1 ;; map_fixvar f c2\<close>
-| \<open>map_fixvar f (c1 \<parallel> c2) = map_fixvar f c1 \<parallel> map_fixvar f c2\<close>
-| \<open>map_fixvar f (c1 \<^bold>+ c2) = map_fixvar f c1 \<^bold>+ map_fixvar f c2\<close>
-| \<open>map_fixvar f (c1 \<box> c2) = map_fixvar f c1 \<box> map_fixvar f c2\<close>
-| \<open>map_fixvar f (DO c OD) = DO (map_fixvar f c) OD\<close>
-| \<open>map_fixvar f (\<mu> c) = \<mu> (map_fixvar (case_nat 0 (Suc \<circ> f)) c)\<close>
-| \<open>map_fixvar f (FixVar x) = FixVar (f x)\<close>
-| \<open>map_fixvar f (Atomic b) = Atomic b\<close>
-
-
-lemma map_fixvar_size[simp]:
-  \<open>size (map_fixvar f c) = size c\<close>
-  by (induct c arbitrary: f) force+
-
-lemma map_fixvar_comp:
-  \<open>map_fixvar f (map_fixvar g c) = map_fixvar (f \<circ> g) c\<close>
-  by (induct c arbitrary: f g)
-    (force intro: arg_cong2[where f=map_fixvar, OF _ refl] simp add: comp_def split: nat.splits)+
-
-lemma map_fixvar_rev_iff:
-  \<open>map_fixvar f c = c1' ;; c2' \<longleftrightarrow>
-    (\<exists>c1 c2. c = c1 ;; c2 \<and> c1' = map_fixvar f c1 \<and> c2' = map_fixvar f c2)\<close>
-  \<open>map_fixvar f c = c1' \<parallel> c2' \<longleftrightarrow>
-      (\<exists>c1 c2. c = c1 \<parallel> c2 \<and> c1' = map_fixvar f c1 \<and> c2' = map_fixvar f c2)\<close>
-  \<open>map_fixvar f c = c1' \<^bold>+ c2' \<longleftrightarrow>
-      (\<exists>c1 c2. c = c1 \<^bold>+ c2 \<and> c1' = map_fixvar f c1 \<and> c2' = map_fixvar f c2)\<close>
-  \<open>map_fixvar f c = c1' \<box> c2' \<longleftrightarrow>
-      (\<exists>c1 c2. c = c1 \<box> c2 \<and> c1' = map_fixvar f c1 \<and> c2' = map_fixvar f c2)\<close>
-  \<open>map_fixvar f c = DO c' OD \<longleftrightarrow>
-      (\<exists>ca. c = DO ca OD \<and> c' = map_fixvar f ca)\<close>
-  \<open>map_fixvar f c = \<mu> c' \<longleftrightarrow>
-      (\<exists>ca. c = \<mu> ca \<and> c' = map_fixvar (case_nat 0 (Suc \<circ> f)) ca)\<close>
-  \<open>map_fixvar f c = Skip \<longleftrightarrow> c = Skip\<close>
-  \<open>map_fixvar f c = FixVar y \<longleftrightarrow> (\<exists>x. c = FixVar x \<and> f x = y)\<close>
-  \<open>map_fixvar f c = Atomic b \<longleftrightarrow> c = Atomic b\<close>
-         apply ((induct c; simp), metis)
-         apply ((induct c; simp), metis)
-        apply ((induct c; simp), metis)
-       apply ((induct c; simp), metis)
-      apply ((induct c; simp), metis)
-     apply ((induct c; simp), blast)
-    apply (induct c; simp; fail)+
-  done
-
-lemmas map_fixvar_sym_rev_iff = map_fixvar_rev_iff[THEN trans[OF eq_commute]]
-
-lemma map_fixvar_inj_inject:
-  \<open>inj f \<Longrightarrow> (map_fixvar f c1 = map_fixvar f c2) = (c1 = c2)\<close>
-proof (induct c1 arbitrary: c2 f)
-  case (Fix c1)
-  moreover have \<open>inj (case_nat 0 (Suc \<circ> f))\<close>
-    using Fix.prems
-    apply (clarsimp simp add: inj_def)
-    apply (case_tac x; case_tac y; simp)
-    done
-  ultimately show ?case
-    by (force simp add: map_fixvar_sym_rev_iff)
-next
-  case (FixVar x)
-  then show ?case
-    by (metis injD map_fixvar_rev_iff(8))
-qed (force simp add: map_fixvar_sym_rev_iff)+
-
-
-primrec fixvar_subst :: \<open>'a comm \<Rightarrow> nat \<Rightarrow> 'a comm \<Rightarrow> 'a comm\<close> (\<open>_[_ \<leftarrow> _]\<close> [1000, 0, 0] 1000) where
-  \<open>Skip[_ \<leftarrow> _] = Skip\<close>
-| \<open>(c1 ;; c2)[x \<leftarrow> c'] = (c1[x \<leftarrow> c'] ;; c2[x \<leftarrow> c'])\<close>
-| \<open>(c1 \<parallel> c2)[x \<leftarrow> c'] = (c1[x \<leftarrow> c'] \<parallel> c2[x \<leftarrow> c'])\<close>
-| \<open>(c1 \<^bold>+ c2)[x \<leftarrow> c'] = (c1[x \<leftarrow> c'] \<^bold>+ c2[x \<leftarrow> c'])\<close>
-| \<open>(c1 \<box> c2)[x \<leftarrow> c'] = (c1[x \<leftarrow> c'] \<box> c2[x \<leftarrow> c'])\<close>
-| \<open>(DO c OD)[x \<leftarrow> c'] = (DO c[x \<leftarrow> c'] OD)\<close>
-| \<open>(\<mu> c)[x \<leftarrow> c'] = \<mu> (c[Suc x \<leftarrow> c'])\<close>
-| \<open>(FixVar y)[x \<leftarrow> c'] = (if x = y then c' else FixVar y)\<close>
-| \<open>(Atomic b)[_ \<leftarrow> _] = Atomic b\<close>
-
-lemma fixvar_subst_rev_iff:
-  \<open>c[x \<leftarrow> cx] = Skip \<longleftrightarrow> c = Skip \<or> c = FixVar x \<and> cx = Skip\<close>
-  \<open>c[x \<leftarrow> cx] = c1' ;; c2' \<longleftrightarrow>
-    (\<exists>c1 c2. c = c1 ;; c2 \<and> c1' = c1[x \<leftarrow> cx] \<and> c2' = c2[x \<leftarrow> cx]) \<or>
-    c = FixVar x \<and> cx = c1' ;; c2'\<close>
-  \<open>c[x \<leftarrow> cx] = c1' \<parallel> c2' \<longleftrightarrow>
-      (\<exists>c1 c2. c = c1 \<parallel> c2 \<and> c1' = c1[x \<leftarrow> cx] \<and> c2' = c2[x \<leftarrow> cx]) \<or>
-      c = FixVar x \<and> cx = c1' \<parallel> c2'\<close>
-  \<open>c[x \<leftarrow> cx] = c1' \<^bold>+ c2' \<longleftrightarrow>
-      (\<exists>c1 c2. c = c1 \<^bold>+ c2 \<and> c1' = c1[x \<leftarrow> cx] \<and> c2' = c2[x \<leftarrow> cx]) \<or>
-      c = FixVar x \<and> cx = c1' \<^bold>+ c2'\<close>
-  \<open>c[x \<leftarrow> cx] = c1' \<box> c2' \<longleftrightarrow>
-      (\<exists>c1 c2. c = c1 \<box> c2 \<and> c1' = c1[x \<leftarrow> cx] \<and> c2' = c2[x \<leftarrow> cx]) \<or>
-      c = FixVar x \<and> cx = c1' \<box> c2'\<close>
-  \<open>c[x \<leftarrow> cx] = DO c' OD \<longleftrightarrow>
-      (\<exists>ca. c = DO ca OD \<and> c' = ca[x \<leftarrow> cx]) \<or>
-      c = FixVar x \<and> cx = DO c' OD\<close>
-  \<open>c[x \<leftarrow> cx] = \<mu> c' \<longleftrightarrow>
-      (\<exists>ca. c = \<mu> ca \<and> c' = ca[Suc x \<leftarrow> cx]) \<or>
-      c = FixVar x \<and> cx = \<mu> c'\<close>
-  \<open>c[x \<leftarrow> cx] = FixVar y \<longleftrightarrow> c = FixVar x \<and> cx = FixVar y \<or> x \<noteq> y \<and> c = FixVar y\<close>
-  \<open>c[x \<leftarrow> cx] = Atomic b \<longleftrightarrow> c = Atomic b \<or> c = FixVar x \<and> cx = Atomic b\<close>
-          apply (induct c; simp; fail)
-         apply ((induct c; simp), metis)+
-  apply (induct c; simp; fail)
-  done
-
-lemma fixvar_subst_over_map_avoid:
-  \<open>\<forall>y. f y \<noteq> x \<Longrightarrow> (map_fixvar f c)[x \<leftarrow> cx] = map_fixvar f c\<close>
-  apply (induct c arbitrary: x f)
-        apply (simp; fail)+
-   apply (drule_tac x=\<open>Suc x\<close> in meta_spec, drule_tac x=\<open>case_nat 0 (Suc \<circ> f)\<close> in meta_spec,
-      clarsimp split: nat.splits)
-  apply force
-  done
-
-subsection \<open> subexpression order \<close>
-
-(*
-instantiation comm :: (type) order
-begin
-
-fun less_eq_comm :: \<open>'a comm \<Rightarrow> 'a comm \<Rightarrow> bool\<close> where
-  \<open>(c \<le> Skip) = (c = Skip)\<close>
-| \<open>(c \<le> c1' ;; c2') = (c = c1' ;; c2' \<or> c \<le> c1' \<or> c \<le> c2')\<close>
-| \<open>(c \<le> c1' \<parallel> c2') = (c = c1' \<parallel> c2' \<or> c \<le> c1' \<or> c \<le> c2')\<close>
-| \<open>(c \<le> c1' \<^bold>+ c2') = (c = c1' \<^bold>+ c2' \<or> c \<le> c1' \<or> c \<le> c2')\<close>
-| \<open>(c \<le> \<mu> c') = (c = \<mu> c' \<or> map_fixvar Suc c \<le> c')\<close>
-| \<open>(c \<le> FixVar x) = (c = FixVar x)\<close>
-| \<open>(c \<le> Atomic b) = (c = Atomic b)\<close>
-
-definition less_comm :: \<open>'a comm \<Rightarrow> 'a comm \<Rightarrow> bool\<close> where
-  \<open>less_comm x y \<equiv> x \<noteq> y \<and> x \<le> y\<close>
-
-lemma less_comm_simps[simp]:
-  \<open>c < Skip \<longleftrightarrow> False\<close>
-  \<open>c < c1' ;; c2' \<longleftrightarrow> c \<noteq> c1' ;; c2' \<and> (c \<le> c1' \<or> c \<le> c2')\<close>
-  \<open>c < c1' \<parallel> c2' \<longleftrightarrow> c \<noteq> c1' \<parallel> c2' \<and> (c \<le> c1' \<or> c \<le> c2')\<close>
-  \<open>c < c1' \<^bold>+ c2' \<longleftrightarrow> c \<noteq> c1' \<^bold>+ c2' \<and> (c \<le> c1' \<or> c \<le> c2')\<close>
-  \<comment> \<open>c < \<mu> c' \<longleftrightarrow> c \<noteq> \<mu> c' \<or> map_fixvar Suc c \<le> c'\<close>
-  \<open>c < FixVar x \<longleftrightarrow> False\<close>
-  \<open>c < Atomic b \<longleftrightarrow> False\<close>
-  by (force simp add: less_comm_def)+
-
-lemma less_eq_comm_refl: \<open>(x::'a comm) \<le> x\<close>
-  by (induct x) force+
-
-lemma less_eq_comm_map_fixvar_inj_mono:
-  \<open>(x::'a comm) \<le> y \<Longrightarrow> inj f \<Longrightarrow> map_fixvar f x \<le> map_fixvar f y\<close>
-  apply (induct y arbitrary: x f)
-        apply force+
-   apply clarsimp
-   apply (erule disjE, force)
-   apply (simp add: map_fixvar_comp comp_def if_distrib[of Suc])
-   apply (case_tac x)
-  oops
-
-lemma less_eq_comm_trans: \<open>(x::'a comm) \<le> y \<Longrightarrow> y \<le> z \<Longrightarrow> x \<le> z\<close>
-  apply (induct z arbitrary: x y) 
-        apply force+
-   apply clarsimp
-   apply (erule disjE, force)
-  oops
-
-lemma less_eq_comm_subexprsD:
-  \<open>(c1 ;; c2) \<le> c \<Longrightarrow> c1 \<le> c\<close>
-  \<open>(c1 ;; c2) \<le> c \<Longrightarrow> c2 \<le> c\<close>
-  \<open>(c1 \<^bold>+ c2) \<le> c \<Longrightarrow> c1 \<le> c\<close>
-  \<open>(c1 \<^bold>+ c2) \<le> c \<Longrightarrow> c2 \<le> c\<close>
-  \<open>(c1 \<parallel> c2) \<le> c \<Longrightarrow> c1 \<le> c\<close>
-  \<open>(c1 \<parallel> c2) \<le> c \<Longrightarrow> c2 \<le> c\<close>
-  \<open>(\<mu> cb) \<le> c \<Longrightarrow> cb \<le> c\<close>
-  (* by (meson less_eq_comm.simps less_eq_comm_refl less_eq_comm_trans; fail)+ *)
-  oops
-
-lemma less_eq_comm_antisym: \<open>(x::'a comm) \<le> y \<Longrightarrow> y \<le> x \<Longrightarrow> x = y\<close>
-  apply (induct y arbitrary: x)
-        apply (simp; fail)+
-(*
-       apply (metis RGLogic.less_eq_comm_subexprsD(1,2) less_eq_comm.simps(2))
-      apply (metis RGLogic.less_eq_comm_subexprsD(5,6) less_eq_comm.simps(3))
-     apply (metis RGLogic.less_eq_comm_subexprsD(3,4) less_eq_comm.simps(4))
-    apply (simp; fail)
-   apply (metis RGLogic.less_eq_comm_subexprsD(7) less_eq_comm.simps(5))
-  apply (simp; fail)
-  done
-*)
-  oops
-
-instance
-  by standard
-    (force intro: less_eq_comm_refl less_eq_comm_trans less_eq_comm_antisym
-      simp add: less_comm_def)+
-
-end
-
-lemma less_eq_comm_no_constructorsD:
-  \<open>(c1 ;; c2) \<le> c \<Longrightarrow> c \<le> c1 \<Longrightarrow> False\<close>
-  \<open>(c1 ;; c2) \<le> c \<Longrightarrow> c \<le> c2 \<Longrightarrow> False\<close>
-  \<open>(c1 \<^bold>+ c2) \<le> c \<Longrightarrow> c \<le> c1 \<Longrightarrow> False\<close>
-  \<open>(c1 \<^bold>+ c2) \<le> c \<Longrightarrow> c \<le> c2 \<Longrightarrow> False\<close>
-  \<open>(c1 \<parallel> c2) \<le> c \<Longrightarrow> c \<le> c1 \<Longrightarrow> False\<close>
-  \<open>(c1 \<parallel> c2) \<le> c \<Longrightarrow> c \<le> c2 \<Longrightarrow> False\<close>
-  \<open>(\<mu> cb) \<le> c \<Longrightarrow> c \<le> cb \<Longrightarrow> False\<close>
-  by (fastforce dest: order.antisym)+
-
-lemma subst_not_subexpr_iff:
-  \<open>\<not> c[x \<leftarrow> cx] \<le> c \<longleftrightarrow> FixVar x \<le> c\<close>
-  apply (induct c)
-        apply force
-       apply clarsimp
-*)
-
-
-subsection \<open> Map atoms \<close>
-
-fun map_comm :: \<open>('b \<Rightarrow> 'a) \<Rightarrow> 'a comm \<Rightarrow> 'b comm\<close> where
-  \<open>map_comm f Skip = Skip\<close>
-| \<open>map_comm f (a ;; b) = map_comm f a ;; map_comm f b\<close>
-| \<open>map_comm f (a \<parallel> b) = map_comm f a \<parallel> map_comm f b\<close>
-| \<open>map_comm f (a \<^bold>+ b) = map_comm f a \<^bold>+ map_comm f b\<close>
-| \<open>map_comm f (a \<box> b) = map_comm f a \<box> map_comm f b\<close>
-| \<open>map_comm f (Atomic b) = Atomic (\<lambda>x y. b (f x) (f y))\<close>
-| \<open>map_comm f (DO a OD) = DO map_comm f a OD\<close>
-| \<open>map_comm f (\<mu> c) = \<mu> (map_comm f c)\<close>
-| \<open>map_comm f (FixVar x) = FixVar x\<close>
-
-lemma map_comm_rev_iff:
-  \<open>map_comm f c = Skip \<longleftrightarrow> c = Skip\<close>
-  \<open>map_comm f c = c1' ;; c2' \<longleftrightarrow>
-    (\<exists>c1 c2. c = c1 ;; c2 \<and> c1' = map_comm f c1 \<and> c2' = map_comm f c2)\<close>
-  \<open>map_comm f c = c1' \<parallel> c2' \<longleftrightarrow>
-      (\<exists>c1 c2. c = c1 \<parallel> c2 \<and> c1' = map_comm f c1 \<and> c2' = map_comm f c2)\<close>
-  \<open>map_comm f c = c1' \<^bold>+ c2' \<longleftrightarrow>
-      (\<exists>c1 c2. c = c1 \<^bold>+ c2 \<and> c1' = map_comm f c1 \<and> c2' = map_comm f c2)\<close>
-  \<open>map_comm f c = c1' \<box> c2' \<longleftrightarrow>
-      (\<exists>c1 c2. c = c1 \<box> c2 \<and> c1' = map_comm f c1 \<and> c2' = map_comm f c2)\<close>
-  \<open>map_comm f c = DO c' OD \<longleftrightarrow>
-      (\<exists>ca. c = DO ca OD \<and> c' = map_comm f ca)\<close>
-  \<open>map_comm f c = \<mu> c' \<longleftrightarrow>
-      (\<exists>ca. c = \<mu> ca \<and> c' = map_comm f ca)\<close>
-  \<open>map_comm f c = FixVar x \<longleftrightarrow> c = FixVar x\<close>
-  \<open>map_comm f c = Atomic b \<longleftrightarrow> (\<exists>b'. c = Atomic b' \<and> b = (\<lambda>x y. b' (f x) (f y)))\<close>
-  by (induct c; simp; argo)+
-
-lemmas map_comm_rev_iff2 = map_comm_rev_iff[THEN trans[OF eq_commute]]
-
-subsection \<open> All atom commands predicate \<close>
-
-text \<open> Predicate to ensure atomic actions have a given property \<close>
-
-inductive all_atom_comm :: \<open>(('a \<Rightarrow> 'a \<Rightarrow> bool) \<Rightarrow> bool) \<Rightarrow> 'a comm \<Rightarrow> bool\<close> where
-  skip[iff]: \<open>all_atom_comm p Skip\<close>
-| seq[intro!]: \<open>all_atom_comm p c1 \<Longrightarrow> all_atom_comm p c2 \<Longrightarrow> all_atom_comm p (c1 ;; c2)\<close>
-| par[intro!]: \<open>all_atom_comm p c1 \<Longrightarrow> all_atom_comm p c2 \<Longrightarrow> all_atom_comm p (c1 \<parallel> c2)\<close>
-| indet[intro!]: \<open>all_atom_comm p c1 \<Longrightarrow> all_atom_comm p c2 \<Longrightarrow> all_atom_comm p (c1 \<^bold>+ c2)\<close>
-| endet[intro!]: \<open>all_atom_comm p c1 \<Longrightarrow> all_atom_comm p c2 \<Longrightarrow> all_atom_comm p (c1 \<box> c2)\<close>
-| iter[intro!]: \<open>all_atom_comm p c \<Longrightarrow> all_atom_comm p (DO c OD)\<close>
-| fixpt[intro!]: \<open>all_atom_comm p c \<Longrightarrow> all_atom_comm p (\<mu> c)\<close>
-| fixvar[iff]: \<open>all_atom_comm p (FixVar x)\<close>
-| atom[intro!]: \<open>p b \<Longrightarrow> all_atom_comm p (Atomic b)\<close>
-
-inductive_cases all_atom_comm_seqE[elim!]: \<open>all_atom_comm p (c1 ;; c2)\<close>
-inductive_cases all_atom_comm_indetE[elim!]: \<open>all_atom_comm p (c1 \<^bold>+ c2)\<close>
-inductive_cases all_atom_comm_endetE[elim!]: \<open>all_atom_comm p (c1 \<box> c2)\<close>
-inductive_cases all_atom_comm_parE[elim!]: \<open>all_atom_comm p (c1 \<parallel> c2)\<close>
-inductive_cases all_atom_comm_iterE[elim!]: \<open>all_atom_comm p (DO c OD)\<close>
-inductive_cases all_atom_comm_fixptE[elim!]: \<open>all_atom_comm p (\<mu> c)\<close>
-inductive_cases all_atom_comm_fixvarE[elim!]: \<open>all_atom_comm p (FixVar x)\<close>
-inductive_cases all_atom_comm_atomE[elim!]: \<open>all_atom_comm p (Atomic b)\<close>
-
-lemma all_atom_comm_simps[simp]:
-  \<open>all_atom_comm p (c1 ;; c2) \<longleftrightarrow> all_atom_comm p c1 \<and> all_atom_comm p c2\<close>
-  \<open>all_atom_comm p (c1 \<^bold>+ c2) \<longleftrightarrow> all_atom_comm p c1 \<and> all_atom_comm p c2\<close>
-  \<open>all_atom_comm p (c1 \<box> c2) \<longleftrightarrow> all_atom_comm p c1 \<and> all_atom_comm p c2\<close>
-  \<open>all_atom_comm p (c1 \<parallel> c2) \<longleftrightarrow> all_atom_comm p c1 \<and> all_atom_comm p c2\<close>
-  \<open>all_atom_comm p (DO c OD) \<longleftrightarrow> all_atom_comm p c\<close>
-  \<open>all_atom_comm p (\<mu> c) \<longleftrightarrow> all_atom_comm p c\<close>
-  \<open>all_atom_comm p (Atomic b) \<longleftrightarrow> p b\<close>
-  by fastforce+
-
-lemma all_atom_comm_pred_mono:
-  \<open>p \<le> q \<Longrightarrow> all_atom_comm p c \<Longrightarrow> all_atom_comm q c\<close>
-  by (induct c) force+
-
-lemma all_atom_comm_pred_mono':
-  \<open>p \<le> q \<Longrightarrow> all_atom_comm p \<le> all_atom_comm q\<close>
-  using all_atom_comm_pred_mono by auto
-
-lemmas all_atom_comm_pred_monoD = all_atom_comm_pred_mono[rotated]
-
-lemma all_atom_comm_conj_eq:
-  \<open>all_atom_comm (p \<sqinter> q) c \<longleftrightarrow> all_atom_comm p c \<and> all_atom_comm q c\<close>
-  by (induct c) force+
-
-lemma all_atom_comm_pconj_eq[simp]:
-  \<open>all_atom_comm (\<lambda>x. p x \<and> q x) c \<longleftrightarrow> all_atom_comm p c \<and> all_atom_comm q c\<close>
-  by (induct c) force+
-
-lemma all_atom_comm_top_eq[simp]:
-  \<open>all_atom_comm \<top> c\<close>
-  by (induct c) force+
-
-lemma all_atom_comm_pTrue_eq[simp]:
-  \<open>all_atom_comm (\<lambda>x. True) c\<close>
-  by (induct c) force+
-
-lemma all_atom_comm_subst[simp]:
-  \<open>all_atom_comm p c' \<Longrightarrow> all_atom_comm p (c[x \<leftarrow> c']) \<longleftrightarrow> all_atom_comm p c\<close>
-  by (induct c arbitrary: x) force+
-
-lemma all_atom_comm_subst_strong:
-  \<open>all_atom_comm p c' - all_atom_comm p c \<Longrightarrow> all_atom_comm p (c[x \<leftarrow> c']) \<longleftrightarrow> all_atom_comm p c\<close>
-  by (induct c arbitrary: x) force+
-
-abbreviation \<open>atoms_subrel_of r \<equiv> all_atom_comm (\<lambda>b. b \<le> r)\<close>
-
-
 section \<open> Rely-Guarantee Separation Logic \<close>
 
 inductive rgsat ::
@@ -564,11 +260,11 @@ inductive rgsat ::
     sswa (r \<squnion> g2) q1 \<^emph>\<and> sswa (r \<squnion> g1) q2 \<le> q \<Longrightarrow>
     rgsat (s1 \<parallel> s2) r g p q\<close>
 | rgsat_atom:
-  \<open>sp b (wssa r p) \<le> sswa r q \<Longrightarrow>
+  \<open>p' \<le> wssa r p \<Longrightarrow>
+    sswa r q \<le> q' \<Longrightarrow>
+    sp b (wssa r p) \<le> sswa r q \<Longrightarrow>
     \<forall>f. sp b (wssa r (p \<^emph>\<and> f)) \<le> sswa r (q \<^emph>\<and> f) \<Longrightarrow>
     b \<le> \<top> \<times>\<^sub>R g \<Longrightarrow>
-    p' \<le> wssa r p \<Longrightarrow>
-    sswa r q \<le> q' \<Longrightarrow>
     rgsat (Atomic b) r g p' q'\<close>
 | rgsat_frame:
   \<open>rgsat c r g p q \<Longrightarrow>
@@ -587,6 +283,11 @@ inductive rgsat ::
     rgsat c r g p2 q2 \<Longrightarrow>
     \<forall>a b c::'l. a ## c \<longrightarrow> b ## c \<longrightarrow> a + c = b + c \<longrightarrow> a = b \<Longrightarrow>
     rgsat c r g (p1 \<sqinter> p2) (q1 \<sqinter> q2)\<close>
+
+abbreviation rgsat_pretty
+  :: \<open>_ \<Rightarrow> _ \<Rightarrow> _ \<Rightarrow> _ \<Rightarrow> _ \<Rightarrow> _\<close>
+  (\<open>_, _ \<turnstile> { _ } _ { _ }\<close> [55, 55, 55, 55, 55] 56) where
+  \<open>r, g \<turnstile> { p } c { q } \<equiv> rgsat c r g p q\<close>
 
 inductive_cases rgsep_doneE[elim]: \<open>rgsat Skip r g p q\<close>
 inductive_cases rgsep_iterE[elim]: \<open>rgsat (DO c OD) r g p q\<close>
