Lang.thy
@@ -1,0 +1,317 @@
+theory Lang
+  imports SepAlgInstances
+begin
+
+
+section \<open> Language Definition \<close>
+
+subsection \<open> Commands \<close>
+
+datatype 'a comm =
+  Skip
+  | Seq \<open>'a comm\<close> \<open>'a comm\<close> (infixr \<open>;;\<close> 75)
+  | Par \<open>'a comm\<close> \<open>'a comm\<close> (infixr \<open>\<parallel>\<close> 65)
+  | Indet \<open>'a comm\<close> \<open>'a comm\<close> (infixr \<open>\<^bold>+\<close> 65)
+  | Endet \<open>'a comm\<close> \<open>'a comm\<close> (infixr \<open>\<box>\<close> 65)
+  | Atomic \<open>'a \<Rightarrow> 'a \<Rightarrow> bool\<close> (\<open>\<langle> _ \<rangle>\<close> [0] 999)
+  | Iter \<open>'a comm\<close> (\<open>DO (_) OD\<close> [0] 999)
+\<comment> \<open> loops are represented by (least) fixed points. Fixed point variables are done in de Brijn
+style. \<close>
+  | Fix \<open>'a comm\<close> (\<open>\<mu>\<close>)
+  | FixVar nat
+
+subsection \<open> substitution \<close>
+
+primrec map_fixvar :: \<open>(nat \<Rightarrow> nat) \<Rightarrow> 'a comm \<Rightarrow> 'a comm\<close> where
+  \<open>map_fixvar f Skip = Skip\<close>
+| \<open>map_fixvar f (c1 ;; c2) = map_fixvar f c1 ;; map_fixvar f c2\<close>
+| \<open>map_fixvar f (c1 \<parallel> c2) = map_fixvar f c1 \<parallel> map_fixvar f c2\<close>
+| \<open>map_fixvar f (c1 \<^bold>+ c2) = map_fixvar f c1 \<^bold>+ map_fixvar f c2\<close>
+| \<open>map_fixvar f (c1 \<box> c2) = map_fixvar f c1 \<box> map_fixvar f c2\<close>
+| \<open>map_fixvar f (DO c OD) = DO (map_fixvar f c) OD\<close>
+| \<open>map_fixvar f (\<mu> c) = \<mu> (map_fixvar (case_nat 0 (Suc \<circ> f)) c)\<close>
+| \<open>map_fixvar f (FixVar x) = FixVar (f x)\<close>
+| \<open>map_fixvar f (Atomic b) = Atomic b\<close>
+
+
+lemma map_fixvar_size[simp]:
+  \<open>size (map_fixvar f c) = size c\<close>
+  by (induct c arbitrary: f) force+
+
+lemma map_fixvar_comp:
+  \<open>map_fixvar f (map_fixvar g c) = map_fixvar (f \<circ> g) c\<close>
+  by (induct c arbitrary: f g)
+    (force intro: arg_cong2[where f=map_fixvar, OF _ refl] simp add: comp_def split: nat.splits)+
+
+lemma map_fixvar_rev_iff:
+  \<open>map_fixvar f c = c1' ;; c2' \<longleftrightarrow>
+    (\<exists>c1 c2. c = c1 ;; c2 \<and> c1' = map_fixvar f c1 \<and> c2' = map_fixvar f c2)\<close>
+  \<open>map_fixvar f c = c1' \<parallel> c2' \<longleftrightarrow>
+      (\<exists>c1 c2. c = c1 \<parallel> c2 \<and> c1' = map_fixvar f c1 \<and> c2' = map_fixvar f c2)\<close>
+  \<open>map_fixvar f c = c1' \<^bold>+ c2' \<longleftrightarrow>
+      (\<exists>c1 c2. c = c1 \<^bold>+ c2 \<and> c1' = map_fixvar f c1 \<and> c2' = map_fixvar f c2)\<close>
+  \<open>map_fixvar f c = c1' \<box> c2' \<longleftrightarrow>
+      (\<exists>c1 c2. c = c1 \<box> c2 \<and> c1' = map_fixvar f c1 \<and> c2' = map_fixvar f c2)\<close>
+  \<open>map_fixvar f c = DO c' OD \<longleftrightarrow>
+      (\<exists>ca. c = DO ca OD \<and> c' = map_fixvar f ca)\<close>
+  \<open>map_fixvar f c = \<mu> c' \<longleftrightarrow>
+      (\<exists>ca. c = \<mu> ca \<and> c' = map_fixvar (case_nat 0 (Suc \<circ> f)) ca)\<close>
+  \<open>map_fixvar f c = Skip \<longleftrightarrow> c = Skip\<close>
+  \<open>map_fixvar f c = FixVar y \<longleftrightarrow> (\<exists>x. c = FixVar x \<and> f x = y)\<close>
+  \<open>map_fixvar f c = Atomic b \<longleftrightarrow> c = Atomic b\<close>
+         apply ((induct c; simp), metis)
+         apply ((induct c; simp), metis)
+        apply ((induct c; simp), metis)
+       apply ((induct c; simp), metis)
+      apply ((induct c; simp), metis)
+     apply ((induct c; simp), blast)
+    apply (induct c; simp; fail)+
+  done
+
+lemmas map_fixvar_sym_rev_iff = map_fixvar_rev_iff[THEN trans[OF eq_commute]]
+
+lemma map_fixvar_inj_inject:
+  \<open>inj f \<Longrightarrow> (map_fixvar f c1 = map_fixvar f c2) = (c1 = c2)\<close>
+proof (induct c1 arbitrary: c2 f)
+  case (Fix c1)
+  moreover have \<open>inj (case_nat 0 (Suc \<circ> f))\<close>
+    using Fix.prems
+    apply (clarsimp simp add: inj_def)
+    apply (case_tac x; case_tac y; simp)
+    done
+  ultimately show ?case
+    by (force simp add: map_fixvar_sym_rev_iff)
+next
+  case (FixVar x)
+  then show ?case
+    by (metis injD map_fixvar_rev_iff(8))
+qed (force simp add: map_fixvar_sym_rev_iff)+
+
+
+primrec fixvar_subst :: \<open>'a comm \<Rightarrow> nat \<Rightarrow> 'a comm \<Rightarrow> 'a comm\<close> (\<open>_[_ \<leftarrow> _]\<close> [1000, 0, 0] 1000) where
+  \<open>Skip[_ \<leftarrow> _] = Skip\<close>
+| \<open>(c1 ;; c2)[x \<leftarrow> c'] = (c1[x \<leftarrow> c'] ;; c2[x \<leftarrow> c'])\<close>
+| \<open>(c1 \<parallel> c2)[x \<leftarrow> c'] = (c1[x \<leftarrow> c'] \<parallel> c2[x \<leftarrow> c'])\<close>
+| \<open>(c1 \<^bold>+ c2)[x \<leftarrow> c'] = (c1[x \<leftarrow> c'] \<^bold>+ c2[x \<leftarrow> c'])\<close>
+| \<open>(c1 \<box> c2)[x \<leftarrow> c'] = (c1[x \<leftarrow> c'] \<box> c2[x \<leftarrow> c'])\<close>
+| \<open>(DO c OD)[x \<leftarrow> c'] = (DO c[x \<leftarrow> c'] OD)\<close>
+| \<open>(\<mu> c)[x \<leftarrow> c'] = \<mu> (c[Suc x \<leftarrow> c'])\<close>
+| \<open>(FixVar y)[x \<leftarrow> c'] = (if x = y then c' else FixVar y)\<close>
+| \<open>(Atomic b)[_ \<leftarrow> _] = Atomic b\<close>
+
+lemma fixvar_subst_rev_iff:
+  \<open>c[x \<leftarrow> cx] = Skip \<longleftrightarrow> c = Skip \<or> c = FixVar x \<and> cx = Skip\<close>
+  \<open>c[x \<leftarrow> cx] = c1' ;; c2' \<longleftrightarrow>
+    (\<exists>c1 c2. c = c1 ;; c2 \<and> c1' = c1[x \<leftarrow> cx] \<and> c2' = c2[x \<leftarrow> cx]) \<or>
+    c = FixVar x \<and> cx = c1' ;; c2'\<close>
+  \<open>c[x \<leftarrow> cx] = c1' \<parallel> c2' \<longleftrightarrow>
+      (\<exists>c1 c2. c = c1 \<parallel> c2 \<and> c1' = c1[x \<leftarrow> cx] \<and> c2' = c2[x \<leftarrow> cx]) \<or>
+      c = FixVar x \<and> cx = c1' \<parallel> c2'\<close>
+  \<open>c[x \<leftarrow> cx] = c1' \<^bold>+ c2' \<longleftrightarrow>
+      (\<exists>c1 c2. c = c1 \<^bold>+ c2 \<and> c1' = c1[x \<leftarrow> cx] \<and> c2' = c2[x \<leftarrow> cx]) \<or>
+      c = FixVar x \<and> cx = c1' \<^bold>+ c2'\<close>
+  \<open>c[x \<leftarrow> cx] = c1' \<box> c2' \<longleftrightarrow>
+      (\<exists>c1 c2. c = c1 \<box> c2 \<and> c1' = c1[x \<leftarrow> cx] \<and> c2' = c2[x \<leftarrow> cx]) \<or>
+      c = FixVar x \<and> cx = c1' \<box> c2'\<close>
+  \<open>c[x \<leftarrow> cx] = DO c' OD \<longleftrightarrow>
+      (\<exists>ca. c = DO ca OD \<and> c' = ca[x \<leftarrow> cx]) \<or>
+      c = FixVar x \<and> cx = DO c' OD\<close>
+  \<open>c[x \<leftarrow> cx] = \<mu> c' \<longleftrightarrow>
+      (\<exists>ca. c = \<mu> ca \<and> c' = ca[Suc x \<leftarrow> cx]) \<or>
+      c = FixVar x \<and> cx = \<mu> c'\<close>
+  \<open>c[x \<leftarrow> cx] = FixVar y \<longleftrightarrow> c = FixVar x \<and> cx = FixVar y \<or> x \<noteq> y \<and> c = FixVar y\<close>
+  \<open>c[x \<leftarrow> cx] = Atomic b \<longleftrightarrow> c = Atomic b \<or> c = FixVar x \<and> cx = Atomic b\<close>
+          apply (induct c; simp; fail)
+         apply ((induct c; simp), metis)+
+  apply (induct c; simp; fail)
+  done
+
+lemma fixvar_subst_over_map_avoid:
+  \<open>\<forall>y. f y \<noteq> x \<Longrightarrow> (map_fixvar f c)[x \<leftarrow> cx] = map_fixvar f c\<close>
+  apply (induct c arbitrary: x f)
+        apply (simp; fail)+
+   apply (drule_tac x=\<open>Suc x\<close> in meta_spec, drule_tac x=\<open>case_nat 0 (Suc \<circ> f)\<close> in meta_spec,
+      clarsimp split: nat.splits)
+  apply force
+  done
+
+subsection \<open> Map atoms \<close>
+
+fun map_comm :: \<open>('b \<Rightarrow> 'a) \<Rightarrow> 'a comm \<Rightarrow> 'b comm\<close> where
+  \<open>map_comm f Skip = Skip\<close>
+| \<open>map_comm f (a ;; b) = map_comm f a ;; map_comm f b\<close>
+| \<open>map_comm f (a \<parallel> b) = map_comm f a \<parallel> map_comm f b\<close>
+| \<open>map_comm f (a \<^bold>+ b) = map_comm f a \<^bold>+ map_comm f b\<close>
+| \<open>map_comm f (a \<box> b) = map_comm f a \<box> map_comm f b\<close>
+| \<open>map_comm f (Atomic b) = Atomic (\<lambda>x y. b (f x) (f y))\<close>
+| \<open>map_comm f (DO a OD) = DO map_comm f a OD\<close>
+| \<open>map_comm f (\<mu> c) = \<mu> (map_comm f c)\<close>
+| \<open>map_comm f (FixVar x) = FixVar x\<close>
+
+lemma map_comm_rev_iff:
+  \<open>map_comm f c = Skip \<longleftrightarrow> c = Skip\<close>
+  \<open>map_comm f c = c1' ;; c2' \<longleftrightarrow>
+    (\<exists>c1 c2. c = c1 ;; c2 \<and> c1' = map_comm f c1 \<and> c2' = map_comm f c2)\<close>
+  \<open>map_comm f c = c1' \<parallel> c2' \<longleftrightarrow>
+      (\<exists>c1 c2. c = c1 \<parallel> c2 \<and> c1' = map_comm f c1 \<and> c2' = map_comm f c2)\<close>
+  \<open>map_comm f c = c1' \<^bold>+ c2' \<longleftrightarrow>
+      (\<exists>c1 c2. c = c1 \<^bold>+ c2 \<and> c1' = map_comm f c1 \<and> c2' = map_comm f c2)\<close>
+  \<open>map_comm f c = c1' \<box> c2' \<longleftrightarrow>
+      (\<exists>c1 c2. c = c1 \<box> c2 \<and> c1' = map_comm f c1 \<and> c2' = map_comm f c2)\<close>
+  \<open>map_comm f c = DO c' OD \<longleftrightarrow>
+      (\<exists>ca. c = DO ca OD \<and> c' = map_comm f ca)\<close>
+  \<open>map_comm f c = \<mu> c' \<longleftrightarrow>
+      (\<exists>ca. c = \<mu> ca \<and> c' = map_comm f ca)\<close>
+  \<open>map_comm f c = FixVar x \<longleftrightarrow> c = FixVar x\<close>
+  \<open>map_comm f c = Atomic b \<longleftrightarrow> (\<exists>b'. c = Atomic b' \<and> b = (\<lambda>x y. b' (f x) (f y)))\<close>
+  by (induct c; simp; argo)+
+
+lemmas map_comm_rev_iff2 = map_comm_rev_iff[THEN trans[OF eq_commute]]
+
+subsection \<open> All atom commands predicate \<close>
+
+text \<open> Predicate to ensure atomic actions have a given property \<close>
+
+inductive all_atom_comm :: \<open>(('a \<Rightarrow> 'a \<Rightarrow> bool) \<Rightarrow> bool) \<Rightarrow> 'a comm \<Rightarrow> bool\<close> where
+  skip[iff]: \<open>all_atom_comm p Skip\<close>
+| seq[intro!]: \<open>all_atom_comm p c1 \<Longrightarrow> all_atom_comm p c2 \<Longrightarrow> all_atom_comm p (c1 ;; c2)\<close>
+| par[intro!]: \<open>all_atom_comm p c1 \<Longrightarrow> all_atom_comm p c2 \<Longrightarrow> all_atom_comm p (c1 \<parallel> c2)\<close>
+| indet[intro!]: \<open>all_atom_comm p c1 \<Longrightarrow> all_atom_comm p c2 \<Longrightarrow> all_atom_comm p (c1 \<^bold>+ c2)\<close>
+| endet[intro!]: \<open>all_atom_comm p c1 \<Longrightarrow> all_atom_comm p c2 \<Longrightarrow> all_atom_comm p (c1 \<box> c2)\<close>
+| iter[intro!]: \<open>all_atom_comm p c \<Longrightarrow> all_atom_comm p (DO c OD)\<close>
+| fixpt[intro!]: \<open>all_atom_comm p c \<Longrightarrow> all_atom_comm p (\<mu> c)\<close>
+| fixvar[iff]: \<open>all_atom_comm p (FixVar x)\<close>
+| atom[intro!]: \<open>p b \<Longrightarrow> all_atom_comm p (Atomic b)\<close>
+
+inductive_cases all_atom_comm_seqE[elim!]: \<open>all_atom_comm p (c1 ;; c2)\<close>
+inductive_cases all_atom_comm_indetE[elim!]: \<open>all_atom_comm p (c1 \<^bold>+ c2)\<close>
+inductive_cases all_atom_comm_endetE[elim!]: \<open>all_atom_comm p (c1 \<box> c2)\<close>
+inductive_cases all_atom_comm_parE[elim!]: \<open>all_atom_comm p (c1 \<parallel> c2)\<close>
+inductive_cases all_atom_comm_iterE[elim!]: \<open>all_atom_comm p (DO c OD)\<close>
+inductive_cases all_atom_comm_fixptE[elim!]: \<open>all_atom_comm p (\<mu> c)\<close>
+inductive_cases all_atom_comm_fixvarE[elim!]: \<open>all_atom_comm p (FixVar x)\<close>
+inductive_cases all_atom_comm_atomE[elim!]: \<open>all_atom_comm p (Atomic b)\<close>
+
+lemma all_atom_comm_simps[simp]:
+  \<open>all_atom_comm p (c1 ;; c2) \<longleftrightarrow> all_atom_comm p c1 \<and> all_atom_comm p c2\<close>
+  \<open>all_atom_comm p (c1 \<^bold>+ c2) \<longleftrightarrow> all_atom_comm p c1 \<and> all_atom_comm p c2\<close>
+  \<open>all_atom_comm p (c1 \<box> c2) \<longleftrightarrow> all_atom_comm p c1 \<and> all_atom_comm p c2\<close>
+  \<open>all_atom_comm p (c1 \<parallel> c2) \<longleftrightarrow> all_atom_comm p c1 \<and> all_atom_comm p c2\<close>
+  \<open>all_atom_comm p (DO c OD) \<longleftrightarrow> all_atom_comm p c\<close>
+  \<open>all_atom_comm p (\<mu> c) \<longleftrightarrow> all_atom_comm p c\<close>
+  \<open>all_atom_comm p (Atomic b) \<longleftrightarrow> p b\<close>
+  by fastforce+
+
+lemma all_atom_comm_pred_mono:
+  \<open>p \<le> q \<Longrightarrow> all_atom_comm p c \<Longrightarrow> all_atom_comm q c\<close>
+  by (induct c) force+
+
+lemma all_atom_comm_pred_mono':
+  \<open>p \<le> q \<Longrightarrow> all_atom_comm p \<le> all_atom_comm q\<close>
+  using all_atom_comm_pred_mono by auto
+
+lemmas all_atom_comm_pred_monoD = all_atom_comm_pred_mono[rotated]
+
+lemma all_atom_comm_conj_eq:
+  \<open>all_atom_comm (p \<sqinter> q) c \<longleftrightarrow> all_atom_comm p c \<and> all_atom_comm q c\<close>
+  by (induct c) force+
+
+lemma all_atom_comm_pconj_eq[simp]:
+  \<open>all_atom_comm (\<lambda>x. p x \<and> q x) c \<longleftrightarrow> all_atom_comm p c \<and> all_atom_comm q c\<close>
+  by (induct c) force+
+
+lemma all_atom_comm_top_eq[simp]:
+  \<open>all_atom_comm \<top> c\<close>
+  by (induct c) force+
+
+lemma all_atom_comm_pTrue_eq[simp]:
+  \<open>all_atom_comm (\<lambda>x. True) c\<close>
+  by (induct c) force+
+
+lemma all_atom_comm_subst[simp]:
+  \<open>all_atom_comm p c' \<Longrightarrow> all_atom_comm p (c[x \<leftarrow> c']) \<longleftrightarrow> all_atom_comm p c\<close>
+  by (induct c arbitrary: x) force+
+
+lemma all_atom_comm_subst_strong:
+  \<open>all_atom_comm p c' - all_atom_comm p c \<Longrightarrow> all_atom_comm p (c[x \<leftarrow> c']) \<longleftrightarrow> all_atom_comm p c\<close>
+  by (induct c arbitrary: x) force+
+
+abbreviation \<open>atoms_subrel_of r \<equiv> all_atom_comm (\<lambda>b. b \<le> r)\<close>
+
+
+section \<open> Specific Languages \<close>
+
+
+subsection \<open> Sugared atomic programs \<close>
+
+definition \<open>passert p \<equiv> \<lambda>a b. p a \<and> a = b\<close>
+
+abbreviation \<open>Assert p \<equiv> Atomic (passert p)\<close>
+abbreviation \<open>Assume p \<equiv> Atomic (\<lambda>a. p)\<close>
+
+lemmas Assert_def = arg_cong[where f=Atomic, OF meta_eq_to_obj_eq[OF passert_def]]
+
+lemma passert_simps[simp]:
+  \<open>passert p a b \<longleftrightarrow> p a \<and> b = a\<close>
+  by (force simp add: passert_def)
+
+subsection \<open> If-then-else and While Loops \<close>
+
+definition \<open>IfThenElse p ct cf \<equiv> Assert p ;; ct \<box> Assert (-p) ;; cf\<close>
+definition \<open>WhileLoop p c \<equiv> \<mu> (Assert p ;; map_fixvar Suc c ;; FixVar 0 \<box> Assert (-p))\<close>
+
+lemma IfThenElse_inject[simp]:
+  \<open>IfThenElse p1 ct1 cf1 = IfThenElse p2 ct2 cf2 \<longleftrightarrow> p1 = p2 \<and> ct1 = ct2 \<and> cf1 = cf2\<close>
+  by (simp add: IfThenElse_def passert_def fun_eq_iff, blast)
+
+lemma WhileLoop_inject[simp]:
+  \<open>WhileLoop p1 c1 = WhileLoop p2 c2 \<longleftrightarrow> p1 = p2 \<and> c1 = c2\<close>
+  by (simp add: WhileLoop_def map_fixvar_inj_inject passert_def fun_eq_iff, blast)
+
+lemma IfThenElse_distinct[simp]:
+  \<open>IfThenElse p ct cf \<noteq> Skip\<close>
+  \<open>IfThenElse p ct cf \<noteq> c1 ;; c2\<close>
+  \<open>IfThenElse p ct cf \<noteq> c1 \<parallel> c2\<close>
+  \<open>IfThenElse p ct cf \<noteq> \<mu> c\<close>
+  \<open>IfThenElse p ct cf \<noteq> Atomic b\<close>
+  \<open>Skip \<noteq> IfThenElse p ct cf\<close>
+  \<open>c1 ;; c2 \<noteq> IfThenElse p ct cf\<close>
+  \<open>c1 \<parallel> c2 \<noteq> IfThenElse p ct cf\<close>
+  \<open>\<mu> c \<noteq> IfThenElse p ct cf\<close>
+  \<open>Atomic b \<noteq> IfThenElse p ct cf\<close>
+  by (simp add: IfThenElse_def)+
+
+lemma WhileLoop_distinct[simp]:
+  \<open>WhileLoop p c \<noteq> Skip\<close>
+  \<open>WhileLoop p c \<noteq> c1 \<box> c2\<close>
+  \<open>WhileLoop p c \<noteq> c1 \<parallel> c2\<close>
+  \<open>WhileLoop p c \<noteq> Atomic b\<close>
+  \<open>Skip \<noteq> WhileLoop p c\<close>
+  \<open>c1 \<box> c2 \<noteq> WhileLoop p c\<close>
+  \<open>c1 \<parallel> c2 \<noteq> WhileLoop p c\<close>
+  \<open>Atomic b \<noteq> WhileLoop p c\<close>
+  \<open>WhileLoop p c \<noteq> \<mu> c\<close>
+  \<open>\<mu> c \<noteq> WhileLoop p c\<close>
+           apply (simp add: WhileLoop_def; fail)+
+   apply (rule size_neq_size_imp_neq, simp add: WhileLoop_def)+
+  done
+
+
+subsection \<open> Heaps \<close>
+
+(* TODO *)
+
+subsection \<open> Locked shared state \<close>
+
+definition acquire
+  :: \<open>nat \<Rightarrow> 'a::perm_alg \<times> 'a resources \<Rightarrow> 'a \<times> 'a resources \<Rightarrow> bool\<close>
+  where
+  \<open>acquire lk \<equiv> \<lambda>(l,s) (l',s'). (\<exists>st.
+      s lk = Some (Unlocked st) \<and>
+      l ## st \<and>
+      l' = l + st \<and>
+      s' = s(lk \<mapsto> Locked)
+  )\<close>
+
+
+end
