SepAlgInstances.thy
@@ -874,11 +874,35 @@ definition emp_mfault :: \<open>('a \<Rightarrow> bool) mfault\<close> ("emp\<^s
 
 end
 
-section \<open> Useful Sepalgebra Constructions \<close>
+section \<open> Locked resources \<close>
+(* TODO: this might be better as a datatype *)
+
+type_synonym 'a locked = \<open>munit + 'a\<close>
+
+abbreviation(input) \<open>Locked \<equiv> Inl \<one> :: 'a locked\<close>
+abbreviation(input) \<open>Unlocked x \<equiv> Inr x :: 'a locked\<close>
+
+lemma disjoint_locked_simps[simp]:
+  \<open>\<And>b. Locked ## b \<longleftrightarrow> False\<close>
+  \<open>\<And>a. a ## Locked \<longleftrightarrow> False\<close>
+  \<open>\<And>a b. Unlocked a ## Unlocked b \<longleftrightarrow> a ## b\<close>
+    apply (case_tac b; simp)
+   apply (case_tac a; simp)
+  apply simp
+  done
+
+type_synonym 'a resources = \<open>nat \<rightharpoonup> 'a locked\<close>
+
+
+section \<open> Heaps and Permission-heaps \<close>
 
 type_synonym ('i,'v) heap = \<open>'i \<rightharpoonup> (munit \<times> 'v discr)\<close>
 
 type_synonym ('i,'v) perm_heap = \<open>'i \<rightharpoonup> (rat fperm \<times> 'v discr)\<close>
+
+(* this also works for resources *)
+definition points_to :: \<open>'a \<Rightarrow> 'b \<Rightarrow> ('a \<rightharpoonup> 'b) \<Rightarrow> bool\<close> (infix \<open>\<^bold>\<mapsto>\<close> 55) where
+  \<open>p \<^bold>\<mapsto> v \<equiv> \<lambda>h. h p = Some v\<close>
 
 
 section \<open> Results \<close>
@@ -896,24 +920,5 @@ lemma sepdomeq_fun:
   apply blast
   done
 
-
-section \<open> Locked resources \<close>
-
-type_synonym 'a locked = \<open>munit + 'a\<close>
-
-definition \<open>Locked \<equiv> Inl \<one> :: 'a locked\<close>
-definition \<open>Unlocked x \<equiv> Inr x :: 'a locked\<close>
-
-lemma disjoint_locked_simps[simp]:
-  \<open>\<And>b. Locked ## b \<longleftrightarrow> False\<close>
-  \<open>\<And>a. a ## Locked \<longleftrightarrow> False\<close>
-  \<open>\<And>a b. Unlocked a ## Unlocked b \<longleftrightarrow> a ## b\<close>
-  unfolding Locked_def Unlocked_def
-    apply (case_tac b; simp)
-   apply (case_tac a; simp)
-  apply simp
-  done
-
-type_synonym 'a resources = \<open>nat \<Rightarrow> 'a locked\<close>
 
 end
